# Biconditionals

<div class="def">

**Converse**: *The implication \\(Q \implies P\\) is called the **converse** of the implication \\(P \implies Q\\).*
* True for open sentences too!
</div>


<h2><center>

**Note!**</h2>

<center>

\\(P \implies Q\\) and \\(P \implies Q\\) have no logical connection!
</center>

<div class="def">

**The Double Implication (biconditional)**

\\[
    P \iff Q \overset{def}{=} (P \implies Q) \ \wedge (Q \implies P)
\\]

</div>

We say:
* \\(P \iff Q\\)
* \\(P\\) is equivalent to \\(Q\\)
* \\(P\\) if and only if \\(Q\\)
* \\(P\\) iff \\(Q\\)
* Older: \\(P\\) is necessary and sufficient for \\(Q\\)

Whenever you're given an English phrasing for double implication, <u>immediately</u> replace it by \\(\iff\\) and proceed from there.

**IMPORTANT**: \\(P \iff Q = T\\) for \\(P, Q = (T, T)\\) **OR** \\(P, Q = (F, F)\\)