# Fundamental Properties of Logical Equivalence

<div class="theorem">

### Theorem 2.18 - Fundamental Logical Equivalences
1. - \\((P \vee Q) \iff (Q \vee P)\\)
   - \\((P \wedge Q) \iff (Q \wedge P)\\)
2. - \\(P \vee (Q \vee R) \iff (P \vee Q) \vee R\\)
   - \\(P \wedge (Q \wedge R) \iff (P \wedge Q) \wedge R\\)
3. - \\(P \vee (Q \wedge R) \iff (P \vee Q) \wedge (P \vee R)\\)
   - \\(P \wedge (Q \vee R) \iff (P \wedge Q) \vee (P \wedge R)\\)
4. - \\(\neg{(P \vee Q)} \iff (\neg{P}) \wedge (\neg{Q})\\)
   - \\(\neg{(P \wedge Q)} \iff (\neg{P}) \vee (\neg{Q})\\)

<!-- **Example**: Prove 

\\[
   \overbar{(P \implies Q)
\\] -->

**Example:** Write negations of the following open sentences:
   * internet was unstable during lecture, couldn't get these copied down. should be in recording from September 1st!