# Proof by Contrapositive

<div class="def">

**Contrapositive**: *The contrapositive of \\(P(x) \implies Q(x)\\) is the implication \\(\neg Q(x) \implies \neg P(x)\\)*
</div>

**Fact**: \\(P(x) \implies Q(x) \iff \left[ \neg Q(x) \implies \neg P(x)\right]\\)

**Proof:**

| \\(P(x)\\) | \\(Q(x)\\) | \\(\neg P(x)\\) | \\(\neg Q(x)\\) | \\(P(x) \implies Q(x)\\) | \\(\neg Q(x) \implies \neg P(x)\\) |
| ---------- | ---------- | --------------- | --------------- | ------------------------ | ---------------------------------- |
| T          | T          | F               | F               | T                        | T                                  |
| T          | F          | F               | T               | F                        | F                                  |
| F          | T          | T               | F               | T                        | T                                  |
| F          | F          | T               | T               | T                        | T                                  |

This results in a proof technique called **proof by contrapositive.**

**Result 3.10:** let \\(x \in \mathbb{Z}\\). If \\(5x-7\\) is even, then \\(x\\) is odd.

**Proof (Contrapositive):** 
* Assume \\(x\\) is even, so \\(x = 2k, k \in \mathbb{Z}\\).
* We want to show that given \\(x\\) is even, then \\(5x-7\\) is odd (\\(5x-7 = 2n+1, n \in \mathbb{Z}\\)).
* Observe: \\[
    \\begin{align}
        5x-7 &= 5(2k)-7\\\\
        &= 2(5k)-8 + 1\\\\
        &= 2(5k-4) + 1
    \\end{align}
\\]
* So, \\(5x-7\\) is odd. \\(\blacksquare\\)

The contrapositive is often used when the hypothesis is difficult, but the conclusion is relatively simple.

### Words of Conclusion
So, thus, therefore, hence, whence, thence, then, it follows that, we have, ...

**Result:** let \\(x \in \mathbb{Z}\\).
\\[
    x -7 \text{ is even} \iff x \text{ is odd.}
\\]

**Proof:** 
* Assume \\(x\\) is odd. Then \\(x = 2k+1, k \in \mathbb{Z}\\).
* We want to show that \\(11x-7 = 2a, a \in \mathbb{Z}\\).
* Observe:
\\[
    \\begin{align}
        11x - 7 &= 11(2k+1) - 7\\\\
        &= 2(11k+11) + 11 - 7\\\\
        &= 2(11k) + 4\\\\
        &= 2(11k+2)\\\\
    \\end{align}
\\]
* So \\(11x-7\\) is even.

For the forward direction, we'll prove by contrapositive.
* Assume \\(x\\) is *even*, so \\(x = 2k, k \in \mathbb{Z}\\).
* We want to show that \\(11x-7 = 2a+1, a \in \mathbb{Z}\\).
* Observe:
\\[
    \\begin{align}
        11x-7 &= 11(2k)-7\\\\
        &= 2(11k) - 8 + 1\\\\
        &= 2(11k-4)+1
    \\end{align}
\\]
* So, \\(11x-7\\) is odd. \\(\blacksquare\\)

## Theorem 3.12
* Let \\(x \in \mathbb{Z}\\). \\(x^2\\) is even \\(\iff x\\) is even.
### Proof
* Assume \\(x\\) is even. In other words, \\(x = 2k, k \in \mathbb{Z}\\).
* We want to show that \\(x^2 = 2a, a \in \mathbb{Z}\\).
* Observe:
\\[
    x^2 = (2k)^2 = 2(2k^2)
\\]
* We'll prove the forward direction by contrapositive.
* Assume \\(x\\) is odd. In other words, \\(x = 2k+1, k \in \mathbb{Z}\\).
* We want to show that \\(x^2 = 2a + 1, a \in \mathbb{Z}\\).
* Observe:
\\[
    \\begin{align}
        x^2 &= (2k+1)^2\\\\
        &= 4k^2+4k+1\\\\
        &= 2(2k^2+2k)+1
    \\end{align}
\\]
* So, \\(x^2\\) is odd. \\(\blacksquare\\)

What about \\(x^2\\) is odd \\(\iff x\\) is odd? We just proved that too!

Result to prove: let \\(x \in \mathbb{Z}\\). If \\(5x-7\\) is odd, then \\(9x+2\\) is even.

* Neither a direct proof nor a contrapositive proof *seems* useful, or at least neither seem like a clean approach.
* Technique: Introduce a **lemma**.
  * A lemma helps bridge the gap between hypothesis and conclusion.
  * A lemma is a **separate** result on its own!

**Lemma:** let \\(x \in \mathbb{Z}\\).
* if \\(5x-7\\) is odd, then \\(x\\) is **even**. (invented hypothesis to simplify)
* We'll prove by contrapositive.
* Assume \\(x\\) is odd, so \\(x = 2k+1, k \in \mathbb{Z}\\).
* We want to show that \\(5x-7 = 2a, a \in \mathbb{Z}\\).
* Observe:
\\[
    \\begin{align}
        5x-7 &= 5(2k+1) - 7\\\\
        &= 2(5k)+5 - 7\\\\
        &= 2(5k) - 2\\\\
        &= 2(5k-1)
    \\end{align}
\\]
* So, \\(5x-7\\) is even. \\(\blacksquare\\)

**Result 3.14**: let \\(x \in \mathbb{Z}\\).
* If \\(5x-7\\) is odd, then \\(9x+2\\) is even.
  
**Proof**: Assume \\(5x-7\\) is odd. By the above lemma, \\(x\\) is even.
* So \\(x = 2k, k \in \mathbb{Z}\\).
* We want to show that \\(9x+2 = 2a, a \in \mathbb{Z}\\).
* Observe:

\\[
    \\begin{align}
        9x + 2 &= 9(2k)+2\\\\
        &= 2(9k+1)
    \\end{align}
\\]
* So, \\(9x+2\\) is even. \\(\blacksquare\\)