# Proofs Involving Divisibility of Integers

**Divides**: if \\(a, b \in \mathbb{Z}\\) with \\(a \neq 0\\), we say "\\(a\\) divides \\(b\\)" if \\(\exists c \in \mathbb{Z}: b = ac\\).
* We write \\(a \mid b\\).
* We also say:
  * \\(b\\) is a multiple of \\(a\\).
  * \\(a\\) is a divisor of \\(b\\).
* If \\(a\\) does not divide \\(b\\), we write \\(a \nmid b\\).

* Old: \\(ab\\) even \\(\iff a\\) is even or \\(b\\) is even.
* New: \\(2 \mid ab \iff 2 \mid a \vee 2 \mid b\\)

**Result 4.1**: let \\(a, b, c \in \mathbb{Z}\\) with \\(a \neq 0\\) and \\(b \neq 0\\).
* If \\(a \mid b\\) and \\(b \mid c\\), then \\(a \mid c\\).
* Proof:
  * Assume \\(a \mid b\\) and \\(b \mid c\\).
  * Then \\(b = ax\\) and \\(c = by\\), \\(x, y \in \mathbb{Z}\\).
  * We want to show that \\(a \mid c\\), meaning \\(c = a \cdot \square, \square \in \mathbb{Z}\\).
  * Observe:

\\[
    \\begin{align}
        c = by = (ax)y = a(xy)
    \\end{align}
\\]
  * So \\(a \mid c\\). \\(\blacksquare\\)

**Result 4.3**: let \\(a, b, c, x, y \in \mathbb{Z}\\), where \\(a \neq 0\\).
* If \\(a \mid b\\) and \\(a \mid c\\), then \\(a \mid (bx + cy)\\).
* Proof:
  * Assume \\(a \mid b\\) and \\(a \mid c\\), \\(a \neq 0\\).
  * **Wrong**: Then \\(b = ax\\) and \\(c = ay, x, y \in \mathbb{Z}\\).
    * We've already used \\(x\\) and \\(y!\\)
  * Then \\(b = ar\\) and \\(c = as, r, s \in \mathbb{Z}\\).
  * We want to show that \\(a \mid (bx+cy\\) meaning \\(bx+cy = a \cdot \square, \square \in \mathbb{Z}\\).
  * Observe:

\\[
    \\begin{align}
        bx + cy &= (ar)x+(as)y\\\\
        &= a(rx+sy)
    \\end{align}
\\]
  * So \\(a \mid (bx+cy)\\). \\(\blacksquare\\)

**Result 4.4**: let \\(x \in \mathbb{Z}\\). If \\(2 \mid (x-1)\\), then \\(4 \mid (x-1)\\).
* **Proof:**
* Assume \\(2 \mid (x^2-1)\\).
  * So \\(x^2 - 1 = 2y, y \in \mathbb{Z}\\).
  * We want to show that \\(4 \mid (x^2-1)\\), meaning \\(x^2-1 = 4 \cdot square, \square \in \mathbb{Z}\\).
    * It's not clear what to do here!
    * That indicates that we probably need to try another path.
  * Try isolating the x term: \\(x^2 = 2y+1\\).
    * Notice: \\(2y+1\\) is odd, and we have a theorem saying that \\(r^2\\) odd \\(\iff r\\) odd!
    * This means \\(x\\) is odd.
  * So \\(x = 2u+1, u \in \mathbb{Z}\\).
  * Observe:

\\[
    \\begin{align}
        x^2 - 1 &= (2u+1)^2-1\\\\
        &= 4u^2+4u+1-1\\\\
        &= 4(u^2+u)
    \\end{align}
\\]
  * So \\(4 \mid (x^2-1)\\). \\(\blacksquare\\)

**Result 4.5**: Let \\(x, y \in \mathbb{Z}\\). If \\(3 \nmid xy\\), then \\(3 \nmid x\\) and \\(3 \nmid y\\).

* Proof by Contrapositive
  * Assume \\(~(3 \nmid x)\\) and \\(\neg 3\nmid y\\)
    * \\(3 \mid x\\) or \\(3 \mid y\\).
  * So \\(x = 3s\\) or \\(y = 3t\\), \\(s, t \in \mathbb{Z}\\).
  * We want to show that \\(3 \mid xy\\), meaning \\(xy = 3\square, \square \in \mathbb{Z}\\).
  * WLOG, assume \\(3\mid x\\), meaning \\(x = 3s\\).
  * Observe: \\(xy = (3s)y = 3(sy)\\).
  * So \\(3 \mid xy\\).

**Handy Observations**: let \\(n \in \mathbb{Z}\\).

1. \\(n = 2q\\) or \\(n = 2q+1\\), \\(q \in \mathbb{Z}\\).
2. \\(n = 3q\\) or \\(n = 3q+1\\) or \\(n = 3q+2\\), \\(q \in \mathbb{Z}\\).
3. For multiples of 2, we have 2 sets. Multiples of 3, 3 sets. Multiples of 4?
    * Notice the pattern :)

**Result 4.6** let \\(x \in \mathbb{Z}\\).
* If \\(3 \nmid (x^2-1)\\), then \\(3 \mid x\\).
* Proof by Contrapositive:
  * Assume \\(3 \nmid x\\).
  * So \\(x\\) is not a multiple of 3.
  * So by the **handy observation**, \\(x = 3q+1\\) or \\(x = 3q+2\\), \\(q \in \mathbb{Z}\\).
  * We want to show that \\(3 \mid (x^2-1)\\), meaning \\(x^2-1 = 3\square, \square \in \mathbb{Z}\\).
    * Case 1: \\(x = 3q+1\\)
    \\[
      \\begin{align}
        x^2-1 &= (3q+1)^2 - 1\\\\
        &= 9q^2+6q+1-1\\\\
        &= 3(3q^2+2q)
      \\end{align}
    \\]
      * So \\(3 \mid (x^2 - 1)\\).
    * Case 2: \\(x = 3q+2\\).
\\[
  \\begin{align}
    x^2 - 1 &= (3q+2)^2\\\\
    &= 9q^2 + 12q + 4 - 1\\\\
    &= 9q^2 + 12q + 3\\\\
    = 3(3q^2+4q+1)
  \\end{align}
\\]
      * So \\(3 \mid (x^2-1)\\).
