# Proofs Involving Congruence of Integers

## Motivation
Let \\(x, y \in \mathbb{Z}\\).
* \\(n = 2\\): \\(x, y\\) must have the form \\(2q\\) or \\(2q+1, q \in \mathbb{Z}\\).
  * Observe: \\(x - y = \\{2a-2b, (2a+1) - (2b+1)\\} = 2(a-b)\\).
* \\(n = 3\\): \\(x, y\\) must have the form \\(3q, 3q+1, 3q+2, q \in \mathbb{Z}\\).
  * Observe: \\(x - y = \\{3a-3b, (3a+1)-(3b+1), (3a+2)-(3b+2)\\} = 3(a-b)\\).

For \\(a, b, n \in \mathbb{Z}, n \geq 2\\), we say \\(a\\) is *congruent* to \\(b \pmod n\\) written \\(a \equiv b \pmod n\\)
* "\\(a\\) equals \\(b\\) \\(\pm\\) a multiple of \\(n\\)"
  * means \\(n \mid (a-b)\\).

**New Interpretation**: \\(x \in \mathbb{Z}\\).
* \\(x = 2q\\) or \\(x = 2q+1, q \in \mathbb{Z}\\).
* \\(x \equiv 0 \pmod 2\\) or \\(x \equiv 1 \pmod 2\\).

**Result 4.9**: let \\(a, b, k, n \in \mathbb{Z}, n \geq 2\\).
* If \\(a \equiv b \pmod n\\), then \\(ka \equiv kb \pmod n\\).
* Proof:
  * Assume \\(a \equiv b \pmod n\\).
  * This means \\(n \mid (a - b)\\).
  * Hence \\(a - b = nx, x \in \mathbb{Z}\\).
  * We want to show that \\(ka \equiv kb \pmod n\\), meaning \\(n \mid (ka - kb)\\)
    * hence \\(ka - kb = n\square, \square \in \mathbb{Z}\\).
  * Observe:

\\[
    \\begin{align}
        ka - kb &= k(a - b)\\\\
        &= k(nx)\\\\
        &= n(kx)
    \\end{align}
\\]
  * Thus \\(ka \equiv kb \pmod n\\). \\(\blacksquare\\)

**Result 4.10**: let \\(a, b, c, d, n \in \mathbb{Z}, n \geq 2\\).
* If \\(a \equiv b \pmod n\\) and \\(c \equiv d \pmod n\\)
* Then \\(a + c \equiv b + d \pmod n\\)
* Proof:
  * Assume \\(a \equiv b \pmod n\\) and \\(c \equiv d \pmod n\\).
    * meaning \\(n \mid (a-b)\\) and \\(n \mid (c-d)\\)
  * Hence \\(a - b = nx\\) and \\(c - d = ny, x, y \in \mathbb{Z}\\)
  * We want to show that \\(a + c \equiv b+d \pmod n\\), meaning \\(n \mid \\left[(a+c)-(b+d)\\right]\\)
  * Observe:

\\[
    \\begin{align}
        (a + c) - (b + d) &= (a - b) + (c - d)\\\\
        &= nx + ny\\\\
        &= n(x + y)
    \\end{align}
\\]
  * So \\(a + c \equiv b + d \pmod n\\)

**Result 4.11**: let \\(a, b, c, d, n \in \mathbb{Z}, n \geq 2\\).
* If \\(a \equiv b \pmod n\\) and \\(c \equiv d \pmod n\\)
* Then \\(ac \equiv bd \pmod n\\).
* Proof: Assume \\(a \equiv b \pmod n\\) and \\(c \equiv d \pmod n\\).
* So, \\(a - b = nx\\) and \\(c - d = ny, x, y \in \mathbb{Z}\\).
* We want to show that \\(ac \equiv bd \pmod n\\), so \\(ac-bd = n\square, \square \in \mathbb{Z}\\).
  * we have \\(a = b+nx\\) and \\(c = d+ny\\)
* Observe:

\\[
    \\begin{align}
        ac-bd &= (b+nx)(d+ny)-bd\\\\
        &= bd+bny + nxd + nxny - bd\\\\
        &= n(by+xd+xny)
    \\end{align}
\\]
* So \\(ac \equiv bd \pmod n\\). \\(\blacksquare\\)

**Result 4.12**: let \\(n \in \mathbb{Z}\\).
* If \\(n^2 \not\equiv n \pmod 3\\)
* then \\(n \not\equiv 0 \pmod 3\\) and \\(n \not\equiv 1 \pmod 3\\)
    * For equals:
      * \\(n^2 \neq n \implies [n \neq 0 \wedge n \neq 1]\\) means \\([n = 0\\) or \\(n = 1] \implies n^2=n\\)
* Proof by Contrapositive
  * Assume \\(\neg[n \not\equiv 0 \pmod 3]\\) and \\(n \not\equiv 1 \pmod 3\\).
    * \\(n \equiv 0 \pmod 3\\) OR \\(n \equiv 1 \pmod 3\\).
  * We want to show that \\(n^2 \equiv n \pmod 3\\), so \\(n^2 - n = 3\square, \square \in \mathbb{Z}\\).
  * Case 1: \\(n \equiv 0 \pmod 3\\)
    * So \\(n - 0 = 3k, k \in \mathbb{Z}\\).
    * Observe: \\(n^2 - n = (3k)^2-(3k) = 3(3k^2-k)\\).
    * So \\(n^2 \equiv n \pmod 3\\).
  * Case 2: \\(n \equiv 1 \pmod 3\\).
    * So \\(n - 1 = 3j, j \in \mathbb{Z}\\).
      * \\(n = 1+3j\\).
    * Observe: 
\\[
    \\begin{align}
        n^2-n &= (1+3j)^2 - (1+3j)\\\\
        &= 1 + 6j + 9j^2 - 1 -3j\\\\
        &= 3(2j+3j^2-j)
    \\end{align}
\\]
    * So \\(n^2 \equiv n \pmod 3\\).